Splinter/BranchTreeInterp.i.dfy
@@ -1,0 +1,52 @@
+include "../lib/Base/total_order.i.dfy"
+include "IndirectionTable.i.dfy"
+include "AllocationTable.i.dfy"
+include "AllocationTableMachine.i.dfy"
+include "MsgHistory.i.dfy"
+include "BranchTree.i.dfy"
+include "SplinterTree.i.dfy"
+include "../Spec/Message.s.dfy"
+include "../Spec/Interp.s.dfy"
+
+
+module BranchTreeInterpMod {
+  import opened Options
+  import opened ValueMessage
+  import KeyType
+  import opened InterpMod
+  import opened DiskTypesMod
+  import opened AllocationMod
+  import opened MsgHistoryMod
+  import IndirectionTableMod
+  import opened BranchTreeMod
+  import SplinterTreeMachineMod
+  import Nat_Order
+
+  type Lookup = BranchPath
+
+  //function IMLookup()
+
+  // NOtE: These might not be needed.
+  function IMKey(root: CU, cache: CacheIfc.Variables, key: Key) : Message
+  {
+    if exists msg, sk :: Query(root, cache, key, msg, sk) // always true by invariant
+    then
+      var msg, sk :| Query(root, cache, key, msg, sk);
+      if msg.Some?
+      then
+        msg.value
+      else
+        DefaultMessage()
+    else
+      // We should never get here
+      DefaultMessage()
+  }
+
+  function IM(root : CU, cache: CacheIfc.Variables) : imap<Key, Message>
+  {
+    imap k | true :: IMKey(root, cache, k)
+  }
+
+  function IReadsKey(v: Variables, cache: CacheIfc.Variables, key: Key) : set<CU>
+
+}
