Splinter/BranchTreeStack.i.dfy
@@ -1,0 +1,92 @@
+include "../lib/Base/total_order.i.dfy"
+include "../lib/Base/Maps.i.dfy"
+include "IndirectionTable.i.dfy"
+include "AllocationTable.i.dfy"
+include "AllocationTableMachine.i.dfy"
+include "MsgHistory.i.dfy"
+include "BranchTree.i.dfy"
+include "../Spec/Message.s.dfy"
+include "../Spec/Interp.s.dfy"
+include "BranchTreeInterp.i.dfy"
+include "../lib/Base/Sequences.i.dfy"
+
+
+/*
+ * Module that deals with transforming and using branches into stacks of range CUs
+ *
+ */
+module BranchTreeStackMod {
+  import opened CacheIfc
+  import opened Options
+  import opened ValueMessage
+  import KeyType
+  import opened InterpMod
+  import opened DiskTypesMod
+  import opened AllocationMod
+  import opened MsgHistoryMod
+  import IndirectionTableMod
+  import opened BranchTreeMod
+  import Nat_Order
+  import BranchTreeInterpMod
+  import opened Maps
+  import opened Sequences
+
+  //////////////////////////////////////////////////////////////////////////////
+  // Define a "Stack" of branches, so we can define what it means to extract
+  // the key-message pairs from a stack and compact it into a new branch tree.
+  //////////////////////////////////////////////////////////////////////////////
+  datatype Range = Range(start: Key, end: Key)
+  {
+    predicate Contains(k : Key)
+    {
+       && Keys.lte(start, k)
+       && Keys.lt(k, end)
+    }
+  }
+
+  datatype Ranges = Ranges(rangeSeq : seq<Range>)
+  {
+    predicate Contains(k : Key)
+    {
+      exists i :: 0 <= i < |rangeSeq| && rangeSeq[i].Contains(k)
+    }
+  }
+
+  datatype Slice = Slice(root: CU, ranges: Ranges, cache: CacheIfc.Variables)
+  {
+
+    function Keys() : iset<Key>
+    {
+        iset k | k in BranchTreeInterpMod.IM(root, cache).Keys && ranges.Contains(k)
+    }
+
+    function IM() :  imap<Key, Message>
+    {
+      imap k | k in Keys() :: BranchTreeInterpMod.IM(root, cache)[k]
+    }
+  }
+
+  datatype Stack = StackFrame(slices : seq<Slice>)
+  {
+  }
+
+  function IM(stack : Stack) :  imap<Key, Message>
+    decreases |stack.slices|
+  {
+      if |stack.slices| == 0
+      then
+        imap []
+      else if |stack.slices| == 1
+      then
+        stack.slices[0].IM()
+      else
+         var stk := StackFrame(DropLast(stack.slices));
+         IMapUnionPreferB(IM(stk), Last(stk.slices).IM())
+  }
+
+  // at the we check that the tree is done
+  predicate IsCompaction(stack : Stack, newroot : CU, cache: CacheIfc.Variables)
+  {
+      IM(stack) == BranchTreeInterpMod.IM(newroot, cache)
+  }
+}
